verified/enc_ni.i.dfy
@@ -2,12 +2,12 @@ include "sec_prop.s.dfy"
 include "pagedb.s.dfy"
 include "entry.s.dfy"
 include "sec_prop_util.i.dfy"
-include "enc_conf_entry.i.dfy"
+include "enc_ni_entry.i.dfy"
 
 //-----------------------------------------------------------------------------
 // Confidentiality, Enclaves are NI with other Enclaves 
 //-----------------------------------------------------------------------------
-lemma lemma_enc_conf_ni(s1: state, d1: PageDb, s1': state, d1': PageDb,
+lemma lemma_enc_ni(s1: state, d1: PageDb, s1': state, d1': PageDb,
                         s2: state, d2: PageDb, s2': state, d2': PageDb,
                         atkr: PageNr)
     requires ni_reqs(s1, d1, s1', d1', s2, d2, s2', d2', atkr)
@@ -18,17 +18,17 @@ lemma lemma_enc_conf_ni(s1: state, d1: PageDb, s1': state, d1': PageDb,
     // s.t. (s1, d1) =_{atkr} (s2, d2)
     requires same_call_args(s1, s2)
     requires InsecureMemInvariant(s1, s2) // public input to mapSecure.
-    requires enc_conf_eqpdb(d1, d2, atkr)
+    requires enc_eqpdb(d1, d2, atkr)
     requires (var callno := s1.regs[R0]; var dispPage := s1.regs[R1];
         (callno == KOM_SMC_ENTER  && entering_atkr(d1, d2, dispPage, atkr, false))
-                ==> enc_conf_eq_entry(s1, s2, d1, d2, atkr))
+                ==> s1.conf.nondet == s2.conf.nondet
     requires (var callno := s1.regs[R0]; var dispPage := s1.regs[R1];
         (callno == KOM_SMC_RESUME  && entering_atkr(d1, d2, dispPage, atkr, true))
-                ==> enc_conf_eq_entry(s1, s2, d1, d2, atkr))
+                ==> s1.conf.nondet == s2.conf.nondet
     // then (s1', d1') =_{atkr} (s2', d2')
     ensures !(var callno := s1.regs[R0]; var asp := s1.regs[R1];
         callno == KOM_SMC_STOP && asp == atkr) ==>
-        enc_conf_eqpdb(d1', d2', atkr)
+        enc_eqpdb(d1', d2', atkr)
 {
     reveal_ValidRegState();
     var callno, arg1, arg2, arg3, arg4
@@ -38,48 +38,48 @@ lemma lemma_enc_conf_ni(s1: state, d1: PageDb, s1': state, d1': PageDb,
     if(callno == KOM_SMC_QUERY || callno == KOM_SMC_GETPHYSPAGES){
         assert d1' == d1;
         assert d2' == d2;
-        reveal_enc_conf_eqpdb();
+        reveal_enc_eqpdb();
     }
     else if(callno == KOM_SMC_INIT_ADDRSPACE){
-        lemma_initAddrspace_enc_conf_ni(d1, d1', e1', d2, d2', e2', arg1, arg2, atkr);
+        lemma_initAddrspace_enc_ni(d1, d1', e1', d2, d2', e2', arg1, arg2, atkr);
     }
     else if(callno == KOM_SMC_INIT_DISPATCHER){
-        lemma_initDispatcher_enc_conf_ni(d1, d1', e1', d2, d2', e2', arg1, arg2, arg3, atkr);
+        lemma_initDispatcher_enc_ni(d1, d1', e1', d2, d2', e2', arg1, arg2, arg3, atkr);
     }
     else if(callno == KOM_SMC_INIT_L2PTABLE){
-        lemma_initL2PTable_enc_conf_ni(d1, d1', e1', d2, d2', e2', arg1, arg2, arg3, atkr);
+        lemma_initL2PTable_enc_ni(d1, d1', e1', d2, d2', e2', arg1, arg2, arg3, atkr);
     }
     else if(callno == KOM_SMC_MAP_SECURE){
-        assert enc_conf_eqpdb(d1', d2', atkr) by {
-            reveal_enc_conf_eqpdb();
+        assert enc_eqpdb(d1', d2', atkr) by {
+            reveal_enc_eqpdb();
             var c1 := maybeContentsOfPhysPage(s1, arg4);
             var c2 := maybeContentsOfPhysPage(s2, arg4);
             assert contentsOk(arg4, c1) && contentsOk(arg4, c2);
             lemma_maybeContents_insec_ni(s1, s2, c1, c2, arg4);
             assert c1 == c2;
-            lemma_mapSecure_enc_conf_ni(d1, c1, d1', e1', d2, c2, d2', e2', arg1, arg2, arg3, arg4, atkr);
+            lemma_mapSecure_enc_ni(d1, c1, d1', e1', d2, c2, d2', e2', arg1, arg2, arg3, arg4, atkr);
         }
     }
     else if(callno == KOM_SMC_MAP_INSECURE){
-        lemma_mapInsecure_enc_conf_ni(d1, d1', e1', d2, d2', e2', arg1, arg2, arg3, atkr);
+        lemma_mapInsecure_enc_ni(d1, d1', e1', d2, d2', e2', arg1, arg2, arg3, atkr);
     }
     else if(callno == KOM_SMC_REMOVE){
-        lemma_remove_enc_conf_ni(d1, d1', e1', d2, d2', e2', arg1, atkr);
+        lemma_remove_enc_ni(d1, d1', e1', d2, d2', e2', arg1, atkr);
     }
     else if(callno == KOM_SMC_FINALISE){
-        lemma_finalise_enc_conf_ni(d1, d1', e1', d2, d2', e2', arg1, atkr);
+        lemma_finalise_enc_ni(d1, d1', e1', d2, d2', e2', arg1, atkr);
     }
     else if(callno == KOM_SMC_ENTER){
-        lemma_enter_enc_conf_ni(s1, d1, s1', d1', s2, d2, s2', d2', arg1, arg2, arg3, arg4, atkr);
+        lemma_enter_enc_ni(s1, d1, s1', d1', s2, d2, s2', d2', arg1, arg2, arg3, arg4, atkr);
     }
     else if(callno == KOM_SMC_RESUME){
-        lemma_resume_enc_conf_ni(s1, d1, s1', d1', s2, d2, s2', d2', arg1, atkr);
+        lemma_resume_enc_ni(s1, d1, s1', d1', s2, d2, s2', d2', arg1, atkr);
     }
     else if(callno == KOM_SMC_STOP){
-        lemma_stop_enc_conf_ni(d1, d1', e1', d2, d2', e2', arg1, atkr);
+        lemma_stop_enc_ni(d1, d1', e1', d2, d2', e2', arg1, atkr);
     }
     else {
-        reveal_enc_conf_eqpdb();
+        reveal_enc_eqpdb();
         assert e1' == KOM_ERR_INVALID;
         assert e2' == KOM_ERR_INVALID;
         assert d1' == d1;
@@ -88,7 +88,7 @@ lemma lemma_enc_conf_ni(s1: state, d1: PageDb, s1': state, d1': PageDb,
 }
 
 
-lemma lemma_mapSecure_enc_conf_ni_both_go(d1: PageDb, c1: Maybe<seq<word>>, d1': PageDb, e1':word,
+lemma lemma_mapSecure_enc_ni_both_go(d1: PageDb, c1: Maybe<seq<word>>, d1': PageDb, e1':word,
                                   d2: PageDb, c2: Maybe<seq<word>>, d2': PageDb, e2':word,
                                   page:word, addrspacePage:word, mapping:word, 
                                   physPage: word, atkr: PageNr)
@@ -98,10 +98,10 @@ lemma lemma_mapSecure_enc_conf_ni_both_go(d1: PageDb, c1: Maybe<seq<word>>, d1':
     requires e1' == KOM_ERR_SUCCESS && e2' == KOM_ERR_SUCCESS
     requires smc_mapSecure(d1, page, addrspacePage, mapping, physPage, c1) == (d1', e1')
     requires smc_mapSecure(d2, page, addrspacePage, mapping, physPage, c2) == (d2', e2')
-    requires enc_conf_eqpdb(d1, d2, atkr)
-    ensures  enc_conf_eqpdb(d1', d2', atkr) 
+    requires enc_eqpdb(d1, d2, atkr)
+    ensures  enc_eqpdb(d1', d2', atkr) 
 {
-    reveal_enc_conf_eqpdb();
+    reveal_enc_eqpdb();
     assert d1'[atkr].PageDbEntryTyped? <==> d1[atkr].PageDbEntryTyped?;
     assert d2'[atkr].PageDbEntryTyped? <==> d2[atkr].PageDbEntryTyped?;
     assert d2'[atkr].PageDbEntryTyped? <==> d1'[atkr].PageDbEntryTyped?;
@@ -110,7 +110,7 @@ lemma lemma_mapSecure_enc_conf_ni_both_go(d1: PageDb, c1: Maybe<seq<word>>, d1':
         var data := DataPage(fromJust(c1)); 
         var ap1 := allocatePage(d1, page, addrspacePage, data);
         var ap2 := allocatePage(d2, page, addrspacePage, data);
-        lemma_allocatePage_enc_conf_ni(d1, ap1.0, ap1.1, d2, ap2.0, ap2.1,
+        lemma_allocatePage_enc_ni(d1, ap1.0, ap1.1, d2, ap2.0, ap2.1,
             page, addrspacePage, data, atkr);
         assert ap1.1 == e1';
         assert ap2.1 == e2';
@@ -120,14 +120,14 @@ lemma lemma_mapSecure_enc_conf_ni_both_go(d1: PageDb, c1: Maybe<seq<word>>, d1':
         assert validL2PTE(ap2.0, addrspacePage, l2pte);
         assert d1' == updateL2Pte(ap1.0, addrspacePage, abs_mapping, l2pte); 
         assert d2' == updateL2Pte(ap2.0, addrspacePage, abs_mapping, l2pte); 
-        lemma_updateL2Pte_enc_conf_ni(ap1.0, d1', ap2.0, d2', 
+        lemma_updateL2Pte_enc_ni(ap1.0, d1', ap2.0, d2', 
             addrspacePage, abs_mapping, l2pte, atkr);
     } else {
-       assert enc_conf_eqpdb(d1', d2', atkr);
+       assert enc_eqpdb(d1', d2', atkr);
     }
 }
 
-lemma lemma_mapSecure_enc_conf_ni_one_go(d1: PageDb, c1: Maybe<seq<word>>, d1': PageDb, e1':word,
+lemma lemma_mapSecure_enc_ni_one_go(d1: PageDb, c1: Maybe<seq<word>>, d1': PageDb, e1':word,
                                   d2: PageDb, c2: Maybe<seq<word>>, d2': PageDb, e2':word,
                                   page:word, addrspacePage:word, mapping:word, 
                                   physPage: word, atkr: PageNr)
@@ -137,22 +137,22 @@ lemma lemma_mapSecure_enc_conf_ni_one_go(d1: PageDb, c1: Maybe<seq<word>>, d1': 
     requires e1' == KOM_ERR_SUCCESS && !(e2' == KOM_ERR_SUCCESS)
     requires smc_mapSecure(d1, page, addrspacePage, mapping, physPage, c1) == (d1', e1')
     requires smc_mapSecure(d2, page, addrspacePage, mapping, physPage, c2) == (d2', e2')
-    requires enc_conf_eqpdb(d1, d2, atkr)
-    ensures  enc_conf_eqpdb(d1', d2', atkr)
+    requires enc_eqpdb(d1, d2, atkr)
+    ensures  enc_eqpdb(d1', d2', atkr)
 {
-    reveal_enc_conf_eqpdb();
+    reveal_enc_eqpdb();
     assert d1'[atkr].PageDbEntryTyped? <==> d1[atkr].PageDbEntryTyped?;
     assert d2'[atkr].PageDbEntryTyped? <==> d2[atkr].PageDbEntryTyped?;
     assert d2'[atkr].PageDbEntryTyped? <==> d1'[atkr].PageDbEntryTyped?;
     assert d2' == d2;
     if( d1'[atkr].PageDbEntryTyped? ){
-        assert enc_conf_eqpdb(d1', d2', atkr);
+        assert enc_eqpdb(d1', d2', atkr);
     } else {
-        assert enc_conf_eqpdb(d1', d2', atkr);
+        assert enc_eqpdb(d1', d2', atkr);
     }
 }
 
-lemma lemma_mapSecure_enc_conf_ni(d1: PageDb, c1: Maybe<seq<word>>, d1': PageDb, e1':word,
+lemma lemma_mapSecure_enc_ni(d1: PageDb, c1: Maybe<seq<word>>, d1': PageDb, e1':word,
                                   d2: PageDb, c2: Maybe<seq<word>>, d2': PageDb, e2':word,
                                   page:word, addrspacePage:word, mapping:word, 
                                   physPage: word, atkr: PageNr)
@@ -161,27 +161,27 @@ lemma lemma_mapSecure_enc_conf_ni(d1: PageDb, c1: Maybe<seq<word>>, d1': PageDb,
     requires c1 == c2;
     requires smc_mapSecure(d1, page, addrspacePage, mapping, physPage, c1) == (d1', e1')
     requires smc_mapSecure(d2, page, addrspacePage, mapping, physPage, c2) == (d2', e2')
-    requires enc_conf_eqpdb(d1, d2, atkr)
-    ensures  enc_conf_eqpdb(d1', d2', atkr) 
+    requires enc_eqpdb(d1, d2, atkr)
+    ensures  enc_eqpdb(d1', d2', atkr) 
 {
-    reveal_enc_conf_eqpdb();
+    reveal_enc_eqpdb();
     var go1, go2 := e1' == KOM_ERR_SUCCESS, e2' == KOM_ERR_SUCCESS; 
     if( go1 && go2 ) {
-        assert enc_conf_eqpdb(d1', d2', atkr) by {
-            lemma_mapSecure_enc_conf_ni_both_go(d1, c1, d1', e1',
+        assert enc_eqpdb(d1', d2', atkr) by {
+            lemma_mapSecure_enc_ni_both_go(d1, c1, d1', e1',
                                   d2, c2, d2', e2',
                                   page, addrspacePage, mapping, 
                                   physPage, atkr);
         }
     }
     if( go1 && !go2 ) {
-            lemma_mapSecure_enc_conf_ni_one_go(d1, c1, d1', e1',
+            lemma_mapSecure_enc_ni_one_go(d1, c1, d1', e1',
                                   d2, c2, d2', e2',
                                   page, addrspacePage, mapping, 
                                   physPage, atkr);
     }
     if( !go1 && go2 ) {
-            lemma_mapSecure_enc_conf_ni_one_go(d2, c2, d2', e2',
+            lemma_mapSecure_enc_ni_one_go(d2, c2, d2', e2',
                                   d1, c1, d1', e1',
                                   page, addrspacePage, mapping, 
                                   physPage, atkr);
@@ -189,25 +189,25 @@ lemma lemma_mapSecure_enc_conf_ni(d1: PageDb, c1: Maybe<seq<word>>, d1': PageDb,
     if( !go1 && !go2 ) {
         assert d1' == d1;
         assert d2' == d2;
-        reveal_enc_conf_eqpdb();
-        assert enc_conf_eqpdb(d1', d2', atkr);
+        reveal_enc_eqpdb();
+        assert enc_eqpdb(d1', d2', atkr);
     }
 }
 
-lemma lemma_initAddrspace_enc_conf_ni(d1: PageDb, d1': PageDb, e1':word,
+lemma lemma_initAddrspace_enc_ni(d1: PageDb, d1': PageDb, e1':word,
                                       d2: PageDb, d2': PageDb, e2':word,
                                       addrspacePage:word, l1PTPage:word,
                                       atkr: PageNr)
     requires ni_reqs_(d1, d1', d2, d2', atkr)
     requires smc_initAddrspace(d1, addrspacePage, l1PTPage) == (d1', e1')
     requires smc_initAddrspace(d2, addrspacePage, l1PTPage) == (d2', e2')
-    requires enc_conf_eqpdb(d1, d2, atkr)
-    ensures  enc_conf_eqpdb(d1', d2', atkr) 
+    requires enc_eqpdb(d1, d2, atkr)
+    ensures  enc_eqpdb(d1', d2', atkr) 
 {
-    reveal_enc_conf_eqpdb();
+    reveal_enc_eqpdb();
     //var atkr_asp := d1[atkr].addrspace;
     if( atkr == addrspacePage ) {
-        assert enc_conf_eqpdb(d1', d2', atkr);
+        assert enc_eqpdb(d1', d2', atkr);
         assert e1' == e2';
     } else {
         forall(n : PageNr)
@@ -232,22 +232,22 @@ lemma lemma_initAddrspace_enc_conf_ni(d1: PageDb, d1': PageDb, e1':word,
     }
 }
 
-lemma lemma_initDispatcher_enc_conf_ni(d1: PageDb, d1': PageDb, e1':word,
+lemma lemma_initDispatcher_enc_ni(d1: PageDb, d1': PageDb, e1':word,
                                        d2: PageDb, d2': PageDb, e2':word,
                                        page:word, addrspacePage:word, entrypoint:word,
                                        atkr: PageNr)
     requires ni_reqs_(d1, d1', d2, d2', atkr)
     requires smc_initDispatcher(d1, page, addrspacePage, entrypoint) == (d1', e1')
     requires smc_initDispatcher(d2, page, addrspacePage, entrypoint) == (d2', e2')
-    requires enc_conf_eqpdb(d1, d2, atkr)
-    ensures  enc_conf_eqpdb(d1', d2', atkr) 
+    requires enc_eqpdb(d1, d2, atkr)
+    ensures  enc_eqpdb(d1', d2', atkr) 
 {
-    reveal_enc_conf_eqpdb();
+    reveal_enc_eqpdb();
     if(isAddrspace(d1, addrspacePage) && isAddrspace(d2, addrspacePage)) {
         var disp := Dispatcher(entrypoint, false, initDispCtxt());
         assert allocatePage(d1, page, addrspacePage, disp) == (d1', e1');
         assert allocatePage(d2, page, addrspacePage, disp) == (d2', e2');
-        lemma_allocatePage_enc_conf_ni(d1, d1', e1', d2, d2', e2',
+        lemma_allocatePage_enc_ni(d1, d1', e1', d2, d2', e2',
             page, addrspacePage, disp, atkr);
     }
     // Get dafny to think about these cases:
@@ -263,7 +263,7 @@ predicate l2initgo(e1':word) {
             e1' == KOM_ERR_INVALID_ADDRSPACE)
 }
 
-lemma lemma_initL2PTable_enc_conf_ni_one_go(d1: PageDb, d1': PageDb, e1':word,
+lemma lemma_initL2PTable_enc_ni_one_go(d1: PageDb, d1': PageDb, e1':word,
                                      d2: PageDb, d2': PageDb, e2':word,
                                      page:word, addrspacePage:word, l1index:word,
                                      atkr: PageNr)
@@ -271,39 +271,39 @@ lemma lemma_initL2PTable_enc_conf_ni_one_go(d1: PageDb, d1': PageDb, e1':word,
     requires smc_initL2PTable(d1, page, addrspacePage, l1index) == (d1', e1')
     requires smc_initL2PTable(d2, page, addrspacePage, l1index) == (d2', e2')
     requires l2initgo(e1') && !l2initgo(e2')
-    requires enc_conf_eqpdb(d1, d2, atkr)
-    ensures enc_conf_eqpdb(d1', d2', atkr) 
+    requires enc_eqpdb(d1, d2, atkr)
+    ensures enc_eqpdb(d1', d2', atkr) 
 {
-    reveal_enc_conf_eqpdb();
+    reveal_enc_eqpdb();
     assert d1'[atkr].PageDbEntryTyped? <==> d1[atkr].PageDbEntryTyped?;
     assert d2'[atkr].PageDbEntryTyped? <==> d2[atkr].PageDbEntryTyped?;
     assert d2'[atkr].PageDbEntryTyped? <==> d1'[atkr].PageDbEntryTyped?;
     assert d2' == d2;
     if( d1'[atkr].PageDbEntryTyped? ){
-        assert enc_conf_eqpdb(d1', d2', atkr);
+        assert enc_eqpdb(d1', d2', atkr);
     } else {
-        assert enc_conf_eqpdb(d1', d2', atkr);
+        assert enc_eqpdb(d1', d2', atkr);
     }
 }
 
-lemma lemma_initL2PTable_enc_conf_ni(d1: PageDb, d1': PageDb, e1':word,
+lemma lemma_initL2PTable_enc_ni(d1: PageDb, d1': PageDb, e1':word,
                                      d2: PageDb, d2': PageDb, e2':word,
                                      page:word, addrspacePage:word, l1index:word,
                                      atkr: PageNr)
     requires ni_reqs_(d1, d1', d2, d2', atkr)
     requires smc_initL2PTable(d1, page, addrspacePage, l1index) == (d1', e1')
     requires smc_initL2PTable(d2, page, addrspacePage, l1index) == (d2', e2')
-    requires enc_conf_eqpdb(d1, d2, atkr)
-    ensures enc_conf_eqpdb(d1', d2', atkr) 
+    requires enc_eqpdb(d1, d2, atkr)
+    ensures enc_eqpdb(d1', d2', atkr) 
 {
-    reveal_enc_conf_eqpdb();
+    reveal_enc_eqpdb();
     var ex1_alloc := l2initgo(e1');
     var ex2_alloc := l2initgo(e2');
     if( ex1_alloc && ex2_alloc) {
         var l2pt := L2PTable(SeqRepeat(NR_L2PTES, NoMapping));
         var ap1 := allocatePage(d1, page, addrspacePage, l2pt);
         var ap2 := allocatePage(d2, page, addrspacePage, l2pt);
-        lemma_allocatePage_enc_conf_ni(d1, ap1.0, e1', d2, ap2.0, e2',
+        lemma_allocatePage_enc_ni(d1, ap1.0, e1', d2, ap2.0, e2',
             page, addrspacePage, l2pt, atkr);
         assert ap1.1 != KOM_ERR_SUCCESS ==> ap1.0 == d1;
         assert ap2.1 != KOM_ERR_SUCCESS ==> ap2.0 == d2;
@@ -327,11 +327,11 @@ lemma lemma_initL2PTable_enc_conf_ni(d1: PageDb, d1': PageDb, e1':word,
         }
     }
     if( ex1_alloc  && !ex2_alloc) { 
-        lemma_initL2PTable_enc_conf_ni_one_go(
+        lemma_initL2PTable_enc_ni_one_go(
             d1, d1', e1', d2, d2', e2', page, addrspacePage, l1index, atkr);
     }
     if( !ex1_alloc && ex2_alloc ) {
-        lemma_initL2PTable_enc_conf_ni_one_go(
+        lemma_initL2PTable_enc_ni_one_go(
             d2, d2', e2', d1, d1', e1', page, addrspacePage, l1index, atkr);
     }
     if( !ex1_alloc && !ex2_alloc) { 
@@ -343,48 +343,48 @@ lemma lemma_initL2PTable_enc_conf_ni(d1: PageDb, d1': PageDb, e1':word,
 
 
 
-lemma lemma_mapInsecure_enc_conf_ni(d1: PageDb, d1': PageDb, e1':word,
+lemma lemma_mapInsecure_enc_ni(d1: PageDb, d1': PageDb, e1':word,
                                     d2: PageDb, d2': PageDb, e2':word,
                                     addrspacePage:word, physPage: word, mapping: word,
                                     atkr: PageNr)
     requires ni_reqs_(d1, d1', d2, d2', atkr)
     requires smc_mapInsecure(d1, addrspacePage, physPage, mapping) == (d1', e1')
     requires smc_mapInsecure(d2, addrspacePage, physPage, mapping) == (d2', e2')
-    requires enc_conf_eqpdb(d1, d2, atkr)
-    ensures enc_conf_eqpdb(d1', d2', atkr) 
+    requires enc_eqpdb(d1, d2, atkr)
+    ensures enc_eqpdb(d1', d2', atkr) 
 {
-    reveal_enc_conf_eqpdb();
+    reveal_enc_eqpdb();
     var go1, go2 := e1' == KOM_ERR_SUCCESS, e2' == KOM_ERR_SUCCESS; 
     if( go1 && go2 ) {
-        assert enc_conf_eqpdb(d1', d2', atkr) by {
+        assert enc_eqpdb(d1', d2', atkr) by {
             var abs_mapping := wordToMapping(mapping);
             var l2pte := InsecureMapping(physPage, abs_mapping.perm.w);
             assert d1' == updateL2Pte(d1, addrspacePage, abs_mapping, l2pte); 
             assert d2' == updateL2Pte(d2, addrspacePage, abs_mapping, l2pte); 
-            lemma_updateL2Pte_enc_conf_ni(d1, d1', d2, d2', 
+            lemma_updateL2Pte_enc_ni(d1, d1', d2, d2', 
                 addrspacePage, abs_mapping, l2pte, atkr);
         }
     }
-    if( go1 && !go2 ) { assert enc_conf_eqpdb(d1', d2', atkr); }
-    if( !go1 && go2 ) { assert enc_conf_eqpdb(d1', d2', atkr); }
+    if( go1 && !go2 ) { assert enc_eqpdb(d1', d2', atkr); }
+    if( !go1 && go2 ) { assert enc_eqpdb(d1', d2', atkr); }
     if( !go1 && !go2 ) {
         assert d1' == d1;
         assert d2' == d2;
-        assert enc_conf_eqpdb(d1', d2', atkr);
+        assert enc_eqpdb(d1', d2', atkr);
     }
 }
 
-lemma lemma_remove_enc_conf_ni(d1: PageDb, d1': PageDb, e1':word,
+lemma lemma_remove_enc_ni(d1: PageDb, d1': PageDb, e1':word,
                                d2: PageDb, d2': PageDb, e2':word,
                                page:word,
                                atkr: PageNr)
     requires ni_reqs_(d1, d1', d2, d2', atkr)
     requires smc_remove(d1, page) == (d1', e1')
     requires smc_remove(d2, page) == (d2', e2')
-    requires enc_conf_eqpdb(d1, d2, atkr)
-    ensures  enc_conf_eqpdb(d1', d2', atkr) 
+    requires enc_eqpdb(d1, d2, atkr)
+    ensures  enc_eqpdb(d1', d2', atkr) 
 {
-    reveal_enc_conf_eqpdb();
+    reveal_enc_eqpdb();
     if(!validPageNr(page) || d1[page].PageDbEntryFree? || 
         d2[page].PageDbEntryFree?) {
         assert d1' == d1;
@@ -441,17 +441,17 @@ lemma lemma_remove_enc_conf_ni(d1: PageDb, d1': PageDb, e1':word,
     }
 }
 
-lemma lemma_finalise_enc_conf_ni(d1: PageDb, d1': PageDb, e1':word,
+lemma lemma_finalise_enc_ni(d1: PageDb, d1': PageDb, e1':word,
                                  d2: PageDb, d2': PageDb, e2':word,
                                  addrspacePage:word,
                                  atkr: PageNr)
     requires ni_reqs_(d1, d1', d2, d2', atkr)
     requires smc_finalise(d1, addrspacePage) == (d1', e1')
     requires smc_finalise(d2, addrspacePage) == (d2', e2')
-    requires enc_conf_eqpdb(d1, d2, atkr)
-    ensures  enc_conf_eqpdb(d1', d2', atkr) 
+    requires enc_eqpdb(d1, d2, atkr)
+    ensures  enc_eqpdb(d1', d2', atkr) 
 {
-    reveal_enc_conf_eqpdb();
+    reveal_enc_eqpdb();
     if(atkr == addrspacePage) {
         assert e1' == KOM_ERR_SUCCESS <==> e2' == KOM_ERR_SUCCESS;
         if(e1' == KOM_ERR_SUCCESS){
@@ -473,19 +473,19 @@ lemma lemma_finalise_enc_conf_ni(d1: PageDb, d1': PageDb, e1':word,
     }
 }
 
-lemma lemma_stop_enc_conf_ni(d1: PageDb, d1': PageDb, e1':word,
+lemma lemma_stop_enc_ni(d1: PageDb, d1': PageDb, e1':word,
                              d2: PageDb, d2': PageDb, e2':word,
                              addrspacePage:word,
                              atkr: PageNr)
     requires ni_reqs_(d1, d1', d2, d2', atkr)
     requires smc_stop(d1, addrspacePage) == (d1', e1')
     requires smc_stop(d2, addrspacePage) == (d2', e2')
-    requires enc_conf_eqpdb(d1, d2, atkr)
-    ensures  addrspacePage != atkr ==> enc_conf_eqpdb(d1', d2', atkr) 
+    requires enc_eqpdb(d1, d2, atkr)
+    ensures  addrspacePage != atkr ==> enc_eqpdb(d1', d2', atkr) 
 {
-    reveal_enc_conf_eqpdb();
+    reveal_enc_eqpdb();
     if(atkr == addrspacePage) {
-        assert addrspacePage != atkr ==> enc_conf_eqpdb(d1', d2', atkr); 
+        assert addrspacePage != atkr ==> enc_eqpdb(d1', d2', atkr); 
     } else {
         forall(n : PageNr)
             ensures pgInAddrSpc(d1', n, atkr) <==> pgInAddrSpc(d2', n, atkr)
@@ -495,7 +495,7 @@ lemma lemma_stop_enc_conf_ni(d1: PageDb, d1': PageDb, e1':word,
     }
 }
 
-lemma lemma_allocatePage_enc_conf_ni(d1: PageDb, d1': PageDb, e1':word,
+lemma lemma_allocatePage_enc_ni(d1: PageDb, d1': PageDb, e1':word,
                                      d2: PageDb, d2': PageDb, e2':word,
                                      page: word, addrspacePage: PageNr, entry: PageDbEntryTyped,
                                      atkr: PageNr)
@@ -505,10 +505,10 @@ lemma lemma_allocatePage_enc_conf_ni(d1: PageDb, d1': PageDb, e1':word,
     requires allocatePageEntryValid(entry);
     requires allocatePage(d1, page, addrspacePage, entry) == (d1', e1')
     requires allocatePage(d2, page, addrspacePage, entry) == (d2', e2')
-    requires enc_conf_eqpdb(d1, d2, atkr)
-    ensures  enc_conf_eqpdb(d1', d2', atkr) 
+    requires enc_eqpdb(d1, d2, atkr)
+    ensures  enc_eqpdb(d1', d2', atkr) 
 {
-    reveal_enc_conf_eqpdb();
+    reveal_enc_eqpdb();
     assert allocatePage_inner(d1, page, addrspacePage, entry) == (d1', e1');
     assert allocatePage_inner(d2, page, addrspacePage, entry) == (d2', e2');
     if( atkr == addrspacePage ) {
@@ -572,7 +572,7 @@ lemma lemma_allocatePage_enc_conf_ni(d1: PageDb, d1': PageDb, e1':word,
     }
 }
 
-lemma lemma_updateL2Pte_enc_conf_ni(d1: PageDb, d1': PageDb,
+lemma lemma_updateL2Pte_enc_ni(d1: PageDb, d1': PageDb,
                                     d2: PageDb, d2': PageDb,
                                     a: PageNr, mapping: Mapping, l2e: L2PTE,
                                     atkr: PageNr)
@@ -583,10 +583,10 @@ lemma lemma_updateL2Pte_enc_conf_ni(d1: PageDb, d1': PageDb,
     requires validL2PTE(d1, a, l2e) && validL2PTE(d2, a, l2e)
     requires d1' == updateL2Pte(d1, a, mapping, l2e) 
     requires d2' == updateL2Pte(d2, a, mapping, l2e) 
-    requires enc_conf_eqpdb(d1, d2, atkr)
-    ensures  enc_conf_eqpdb(d1', d2', atkr) 
+    requires enc_eqpdb(d1, d2, atkr)
+    ensures  enc_eqpdb(d1', d2', atkr) 
 {
-    reveal_enc_conf_eqpdb();
+    reveal_enc_eqpdb();
     assert d1[a].addrspace == a;
     assert d2[a].addrspace == a;
     var l11 := d1[d1[a].entry.l1ptnr].entry;
