verified/enc_ni_entry.i.dfy
@@ -6,7 +6,7 @@ include "smcapi.i.dfy"
 
 
 // This one's unstable so it's at the top!
-lemma lemma_userspaceExec_atkr_conf(
+lemma lemma_userspaceExec_atkr(
 s11: state, s1':state, s12: state, s13:state, s14: state, d1:PageDb, d14: PageDb,
 s21: state, s2':state, s22: state, s23:state, s24: state, d2:PageDb, d24: PageDb,
 dispPg: PageNr, atkr: PageNr, l1p: PageNr)
@@ -15,13 +15,13 @@ dispPg: PageNr, atkr: PageNr, l1p: PageNr)
     requires validPageDb(d1) && validPageDb(d14)
     requires validPageDb(d2) && validPageDb(d24)
     requires SaneConstants()
-    requires enc_conf_eq_entry(s12, s22, d1, d2, atkr);
+    requires s12.conf.nondet == s22.conf.nondet;
     requires userspaceExecutionAndException'(s11, s1', s12, s14)
     requires userspaceExecutionAndException'(s21, s2', s22, s24)
     requires s13 == userspaceExecutionFn(s12, OperandContents(s11, OLR)).0;
     requires s23 == userspaceExecutionFn(s22, OperandContents(s21, OLR)).0;
     requires atkr_entry(d1, d2, dispPg, atkr)
-    requires enc_conf_eqpdb(d1, d2, atkr)
+    requires enc_eqpdb(d1, d2, atkr)
     requires l1pOfDispatcher(d1, dispPg) == l1pOfDispatcher(d2, dispPg) == l1p
     requires OperandContents(s11, OLR) == OperandContents(s21, OLR)
     requires user_regs(s11.regs) == user_regs(s21.regs)
@@ -32,11 +32,11 @@ dispPg: PageNr, atkr: PageNr, l1p: PageNr)
         dataPagesCorrespond(s22.m, d2)
     requires d14 == updateUserPagesFromState(s14, d1, dispPg);
     requires d24 == updateUserPagesFromState(s24, d2, dispPg);
-    ensures enc_conf_eqpdb(d14, d24, atkr)
+    ensures enc_eqpdb(d14, d24, atkr)
     ensures atkr_entry(d14, d24, dispPg, atkr)
 {
     // reveal_evalUserspaceExecution();
-    reveal_enc_conf_eqpdb();
+    reveal_enc_eqpdb();
 
     assert validPageDb(d14) && validPageDb(d24);
 
@@ -63,7 +63,7 @@ dispPg: PageNr, atkr: PageNr, l1p: PageNr)
     var pt1 := ExtractAbsPageTable(s12);
     var pt2 := ExtractAbsPageTable(s22);
     
-    lemma_userStatesEquiv_atkr_conf(
+    lemma_userStatesEquiv_atkr(
         s11, s1', s12, s14, pc1, pt1, d1,
         s21, s2', s22, s24, pc2, pt2, d2,
         dispPg, atkr, l1p);
@@ -124,23 +124,23 @@ dispPg: PageNr, atkr: PageNr, l1p: PageNr)
         }
     }
 
-    reveal_enc_conf_eqpdb();
-    assert enc_conf_eqpdb(d14, d24, atkr);
+    reveal_enc_eqpdb();
+    assert enc_eqpdb(d14, d24, atkr);
 }
 
-lemma lemma_enter_enc_conf_ni(s1: state, d1: PageDb, s1':state, d1': PageDb,
+lemma lemma_enter_enc_ni(s1: state, d1: PageDb, s1':state, d1': PageDb,
                               s2: state, d2: PageDb, s2':state, d2': PageDb,
                               dispPage: word, arg1: word, arg2: word, arg3: word,
                               atkr: PageNr)
     requires ni_reqs(s1, d1, s1', d1', s2, d2, s2', d2', atkr)
     requires smc_enter(s1, d1, s1', d1', dispPage, arg1, arg2, arg3)
     requires smc_enter(s2, d2, s2', d2', dispPage, arg1, arg2, arg3)
-    requires enc_conf_eqpdb(d1, d2, atkr)
+    requires enc_eqpdb(d1, d2, atkr)
     requires entering_atkr(d1, d2, dispPage, atkr, false) ==>
-        enc_conf_eq_entry(s1, s2, d1, d2, atkr)
-    ensures enc_conf_eqpdb(d1', d2', atkr)
+        s1.conf.nondet == s2.conf.nondet
+    ensures enc_eqpdb(d1', d2', atkr)
 {
-    reveal_enc_conf_eqpdb();
+    reveal_enc_eqpdb();
     if(!validPageNr(dispPage)){
         assert d1' == d1 &&  d2' == d2;
     } else {
@@ -151,8 +151,8 @@ lemma lemma_enter_enc_conf_ni(s1: state, d1: PageDb, s1':state, d1': PageDb,
             assert d2[dispPage].PageDbEntryTyped?;
             var asp1, asp2 := d1[dispPage].addrspace, d2[dispPage].addrspace;
             var e1', e2' := smc_enter_err(d1, dispPage, false), smc_enter_err(d2, dispPage, false);
-            assert enc_conf_eqpdb(d1', d2', atkr) by {
-                lemma_enter_enc_conf_eqpdb(s1, d1, s1', d1', s2, d2, s2', d2',
+            assert enc_eqpdb(d1', d2', atkr) by {
+                lemma_enter_enc_eqpdb(s1, d1, s1', d1', s2, d2, s2', d2',
                                  dispPage, arg1, arg2, arg3, asp1, asp2, atkr, 
                                  false);
             }
@@ -168,7 +168,7 @@ lemma lemma_enter_enc_conf_ni(s1: state, d1: PageDb, s1':state, d1': PageDb,
                 assert e1' == KOM_ERR_SUCCESS <==> e2' == KOM_ERR_SUCCESS;
                 if(e1' == KOM_ERR_SUCCESS) {
                     assert entering_atkr(d1, d2, dispPage, atkr, false);
-                    lemma_enter_enc_conf_atkr_enter(s1, d1, s1', d1', s2, d2, s2', d2',
+                    lemma_enter_enc_atkr_enter(s1, d1, s1', d1', s2, d2, s2', d2',
                                                     dispPage, arg1, arg2, arg3, 
                                                     atkr, false);
                 } else {
@@ -184,7 +184,7 @@ lemma lemma_enter_enc_conf_ni(s1: state, d1: PageDb, s1':state, d1': PageDb,
 lemma 
 {:fuel outside_world_same, 0}
 {:timeLimitMultiplier 2}
-lemma_enter_enc_conf_eqpdb_not_atkr(s1: state, d1: PageDb, s1':state, d1': PageDb,
+lemma_enter_enc_eqpdb_not_atkr(s1: state, d1: PageDb, s1':state, d1': PageDb,
                                  s2: state, d2: PageDb, s2':state, d2': PageDb,
                                  disp: word, arg1: word, arg2: word, arg3: word,
                                  asp1: PageNr, asp2: PageNr, atkr: PageNr,
@@ -197,14 +197,14 @@ lemma_enter_enc_conf_eqpdb_not_atkr(s1: state, d1: PageDb, s1':state, d1': PageD
     requires validPageNr(disp) && d1[disp].PageDbEntryTyped? && 
         d2[disp].PageDbEntryTyped?
     requires d1[disp].addrspace == asp1 && d2[disp].addrspace == asp2
-    requires enc_conf_eqpdb(d1, d2, atkr)
+    requires enc_eqpdb(d1, d2, atkr)
     requires asp1 != atkr && asp2 != atkr
     requires validPageNr(disp) && valDispPage(d1', disp) && valDispPage(d2', disp)
     requires outside_world_same(d1, d1', disp, asp1)
     requires outside_world_same(d2, d2', disp, asp2)
     requires smc_enter_err(d1, disp, isresume) == KOM_ERR_SUCCESS
             && (smc_enter_err(d2, disp, isresume) == KOM_ERR_SUCCESS);
-    ensures  enc_conf_eqpdb(d1', d2', atkr)
+    ensures  enc_eqpdb(d1', d2', atkr)
 {
 
     assert {:fuel outside_world_same, 1}
@@ -238,16 +238,16 @@ lemma_enter_enc_conf_eqpdb_not_atkr(s1: state, d1: PageDb, s1':state, d1': PageD
             pgInAddrSpc(d1, n, atkr);
         assert forall n : PageNr :: pgInAddrSpc(d2', n, atkr) <==>
             pgInAddrSpc(d2, n, atkr);
-        reveal enc_conf_eqpdb();
+        reveal enc_eqpdb();
     }
 
     assert forall n : PageNr | pgInAddrSpc(d1', n, atkr) ::
-        d1'[n].entry == d2'[n].entry by {reveal enc_conf_eqpdb();}
+        d1'[n].entry == d2'[n].entry by {reveal enc_eqpdb();}
 
     // This times out without DAFNYPROC :(
     // The assert also should not be necessary...
-    assert enc_conf_eqpdb(d1', d2', atkr) by {
-        reveal enc_conf_eqpdb();
+    assert enc_eqpdb(d1', d2', atkr) by {
+        reveal enc_eqpdb();
 
         assert d1'[atkr].PageDbEntryTyped? <==> d2'[atkr].PageDbEntryTyped? &&
         (d1'[atkr].PageDbEntryTyped? ==>
@@ -259,7 +259,7 @@ lemma_enter_enc_conf_eqpdb_not_atkr(s1: state, d1: PageDb, s1':state, d1': PageD
     }
 }
 
-lemma lemma_enter_enc_conf_eqpdb(s1: state, d1: PageDb, s1':state, d1': PageDb,
+lemma lemma_enter_enc_eqpdb(s1: state, d1: PageDb, s1':state, d1': PageDb,
                                  s2: state, d2: PageDb, s2':state, d2': PageDb,
                                  disp: word, arg1: word, arg2: word, arg3: word,
                                  asp1: PageNr, asp2: PageNr, atkr: PageNr,
@@ -272,13 +272,13 @@ lemma lemma_enter_enc_conf_eqpdb(s1: state, d1: PageDb, s1':state, d1': PageDb,
     requires validPageNr(disp) && d1[disp].PageDbEntryTyped? && 
         d2[disp].PageDbEntryTyped?
     requires d1[disp].addrspace == asp1 && d2[disp].addrspace == asp2
-    requires enc_conf_eqpdb(d1, d2, atkr)
+    requires enc_eqpdb(d1, d2, atkr)
     requires entering_atkr(d1, d2, disp, atkr, isresume) ==>
-        enc_conf_eq_entry(s1, s2, d1, d2, atkr)
-    ensures  enc_conf_eqpdb(d1', d2', atkr)
+        s1.conf.nondet == s2.conf.nondet
+    ensures  enc_eqpdb(d1', d2', atkr)
 {
 
-    reveal_enc_conf_eqpdb();
+    reveal_enc_eqpdb();
     var go1 := smc_enter_err(d1, disp, isresume) == KOM_ERR_SUCCESS;
     var go2 := smc_enter_err(d2, disp, isresume) == KOM_ERR_SUCCESS;
 
@@ -303,33 +303,33 @@ lemma lemma_enter_enc_conf_eqpdb(s1: state, d1: PageDb, s1':state, d1': PageDb,
         
         if(asp1 == atkr) {
             assert entering_atkr(d1, d2, disp, atkr, isresume);
-            assert enc_conf_eq_entry(s1, s2, d1, d2, atkr);
-            lemma_enter_enc_conf_atkr_enter(s1, d1, s1', d1', s2, d2, s2', d2',
+            assert s1.conf.nondet == s2.conf.nondet;
+            lemma_enter_enc_atkr_enter(s1, d1, s1', d1', s2, d2, s2', d2',
                                             disp, arg1, arg2, arg3, 
                                             atkr, isresume);
         } else {
-            lemma_enter_enc_conf_eqpdb_not_atkr(s1, d1, s1', d1', s2, d2, s2', d2',
+            lemma_enter_enc_eqpdb_not_atkr(s1, d1, s1', d1', s2, d2, s2', d2',
                          disp, arg1, arg2, arg3, asp1, asp2, atkr, isresume);
         }
     }
 
     if(go1 && !go2) {
-        lemma_enter_enc_conf_eqpdb_one_go(s1, d1, s1', d1', s2, d2, s2', d2',
+        lemma_enter_enc_eqpdb_one_go(s1, d1, s1', d1', s2, d2, s2', d2',
                          disp, arg1, arg2, arg3, asp1, asp2, atkr, isresume);
-        assert enc_conf_eqpdb(d1', d2', atkr);
+        assert enc_eqpdb(d1', d2', atkr);
     }
     if(!go1 && go2) {
-        lemma_enter_enc_conf_eqpdb_one_go(s2, d2, s2', d2', s1, d1, s1', d1',
+        lemma_enter_enc_eqpdb_one_go(s2, d2, s2', d2', s1, d1, s1', d1',
                          disp, arg1, arg2, arg3, asp2, asp1, atkr, isresume);
-        assert enc_conf_eqpdb(d1', d2', atkr);
+        assert enc_eqpdb(d1', d2', atkr);
     }
     if(!go1 && !go2) { 
         assert d1' == d1 && d2' == d2;
-        assert enc_conf_eqpdb(d1', d2', atkr);
+        assert enc_eqpdb(d1', d2', atkr);
     }
 }
 
-lemma lemma_enter_enc_conf_eqpdb_one_go(s1: state, d1: PageDb, s1':state, d1': PageDb,
+lemma lemma_enter_enc_eqpdb_one_go(s1: state, d1: PageDb, s1':state, d1': PageDb,
                                         s2: state, d2: PageDb, s2':state, d2': PageDb,
                                         disp: word, arg1: word, arg2: word, arg3: word,
                                         asp1: PageNr, asp2: PageNr, atkr: PageNr,
@@ -342,12 +342,12 @@ lemma lemma_enter_enc_conf_eqpdb_one_go(s1: state, d1: PageDb, s1':state, d1': P
     requires validPageNr(disp) && d1[disp].PageDbEntryTyped? && 
         d2[disp].PageDbEntryTyped?
     requires d1[disp].addrspace == asp1 && d2[disp].addrspace == asp2
-    requires enc_conf_eqpdb(d1, d2, atkr)
+    requires enc_eqpdb(d1, d2, atkr)
     requires smc_enter_err(d1, disp, isresume) == KOM_ERR_SUCCESS
             && !(smc_enter_err(d2, disp, isresume) == KOM_ERR_SUCCESS);
-    ensures  enc_conf_eqpdb(d1', d2', atkr)
+    ensures  enc_eqpdb(d1', d2', atkr)
 {
-   reveal_enc_conf_eqpdb();
+   reveal_enc_eqpdb();
    var go1 := smc_enter_err(d1, disp, isresume) == KOM_ERR_SUCCESS;
    var go2 := smc_enter_err(d2, disp, isresume) == KOM_ERR_SUCCESS;
    assert go1 && !go2;
@@ -390,9 +390,9 @@ lemma lemma_enter_enc_conf_eqpdb_one_go(s1: state, d1: PageDb, s1':state, d1': P
    assert forall n : PageNr | pgInAddrSpc(d1', n, atkr) ::
        d1'[n].entry == d2'[n].entry;
    
-   assert enc_conf_eqpdb(d1', d2', atkr);
+   assert enc_eqpdb(d1', d2', atkr);
 
-   assert enc_conf_eqpdb(d1', d2', atkr);
+   assert enc_eqpdb(d1', d2', atkr);
 }
 
 //-----------------------------------------------------------------------------
@@ -559,7 +559,7 @@ predicate atkr_entry(d1: PageDb, d2: PageDb, disp: word, atkr: PageNr)
 }
 
 
-lemma lemma_enter_enc_conf_atkr_enter(s1: state, d1: PageDb, s1':state, d1': PageDb,
+lemma lemma_enter_enc_atkr_enter(s1: state, d1: PageDb, s1':state, d1': PageDb,
                                       s2: state, d2: PageDb, s2':state, d2': PageDb,
                                       dispPage: word, arg1: word, arg2: word, arg3: word,
                                       atkr: PageNr, isresume:bool)
@@ -568,10 +568,10 @@ lemma lemma_enter_enc_conf_atkr_enter(s1: state, d1: PageDb, s1':state, d1': Pag
     requires !isresume ==> smc_enter(s2, d2, s2', d2', dispPage, arg1, arg2, arg3)
     requires isresume ==> smc_resume(s1, d1, s1', d1', dispPage)
     requires isresume ==> smc_resume(s2, d2, s2', d2', dispPage)
-    requires enc_conf_eqpdb(d1, d2, atkr)
+    requires enc_eqpdb(d1, d2, atkr)
     requires entering_atkr(d1, d2, dispPage, atkr, isresume);
-    requires enc_conf_eq_entry(s1, s2, d1, d2, atkr)
-    ensures  enc_conf_eqpdb(d1', d2', atkr)
+    requires s1.conf.nondet == s2.conf.nondet
+    ensures  enc_eqpdb(d1', d2', atkr)
 {
 
     if(!isresume) {
@@ -590,7 +590,7 @@ lemma lemma_enter_enc_conf_atkr_enter(s1: state, d1: PageDb, s1':state, d1': Pag
         {
             assert OperandContents(s11, OLR) == d1[dispPage].entry.entrypoint;
             assert OperandContents(s21, OLR) == d2[dispPage].entry.entrypoint;
-            reveal enc_conf_eqpdb();
+            reveal enc_eqpdb();
         }
         
         // assert steps1 == steps2 by {
@@ -626,7 +626,7 @@ lemma lemma_enter_enc_conf_atkr_enter(s1: state, d1: PageDb, s1':state, d1': Pag
                 reveal_BitAnd();
             }
         }
-        lemma_validEnclaveEx_enc_conf(s11, d1, s1', d1', s21, d2, s2', d2',
+        lemma_validEnclaveEx_enc(s11, d1, s1', d1', s21, d2, s2', d2',
                                              dispPage, steps1, steps2, atkr);
     } else {
         var s11:state, steps1: nat :|
@@ -640,7 +640,7 @@ lemma lemma_enter_enc_conf_atkr_enter(s1: state, d1: PageDb, s1':state, d1': Pag
         assert s11.conf.nondet == s21.conf.nondet;
 
         assert d1[dispPage].entry == d2[dispPage].entry by
-            { reveal enc_conf_eqpdb(); }
+            { reveal enc_eqpdb(); }
 
         assert user_regs(s11.regs) == user_regs(s21.regs) by {
             var disp := d1[dispPage].entry;
@@ -654,7 +654,7 @@ lemma lemma_enter_enc_conf_atkr_enter(s1: state, d1: PageDb, s1':state, d1': Pag
         {   
             assert OperandContents(s11, OLR) == d1[dispPage].entry.ctxt.pc;
             assert OperandContents(s21, OLR) == d2[dispPage].entry.ctxt.pc;
-            reveal enc_conf_eqpdb();
+            reveal enc_eqpdb();
         }
         
         // assert steps1 == steps2 by {
@@ -675,12 +675,12 @@ lemma lemma_enter_enc_conf_atkr_enter(s1: state, d1: PageDb, s1':state, d1': Pag
             assert s11.sregs[spsr(mode1)] == disp.ctxt.cpsr;
             assert s21.sregs[spsr(mode2)] == disp.ctxt.cpsr;
         }
-        lemma_validEnclaveEx_enc_conf(s11, d1, s1', d1', s21, d2, s2', d2',
+        lemma_validEnclaveEx_enc(s11, d1, s1', d1', s21, d2, s2', d2',
                                              dispPage, steps1, steps2, atkr);
     }
 }
 
-lemma lemma_validEnclaveEx_enc_conf(s1: state, d1: PageDb, s1':state, d1': PageDb,
+lemma lemma_validEnclaveEx_enc(s1: state, d1: PageDb, s1':state, d1': PageDb,
                                     s2: state, d2: PageDb, s2':state, d2': PageDb,
                                     dispPg: PageNr, steps1:nat, steps2:nat,
                                     atkr: PageNr)
@@ -692,8 +692,8 @@ lemma lemma_validEnclaveEx_enc_conf(s1: state, d1: PageDb, s1':state, d1': PageD
     requires atkr_entry(d1, d2, dispPg, atkr)
     requires validEnclaveExecution(s1, d1, s1', d1', dispPg, steps1)
     requires validEnclaveExecution(s2, d2, s2', d2', dispPg, steps2);
-    requires enc_conf_eqpdb(d1, d2, atkr)
-    requires enc_conf_eq_entry(s1, s2, d1, d2, atkr)
+    requires enc_eqpdb(d1, d2, atkr)
+    requires s1.conf.nondet == s2.conf.nondet
     requires OperandContents(s1, OLR) == OperandContents(s2, OLR)
     requires user_regs(s1.regs) == user_regs(s2.regs)
     requires mode_of_state(s1) != User && mode_of_state(s2) != User
@@ -702,7 +702,7 @@ lemma lemma_validEnclaveEx_enc_conf(s1: state, d1: PageDb, s1':state, d1': PageD
     requires spsr_same(s1, s2)
     requires s1.conf.scr == s2.conf.scr;
     ensures  atkr_entry(d1', d2', dispPg, atkr)
-    ensures  enc_conf_eqpdb(d1', d2', atkr)
+    ensures  enc_eqpdb(d1', d2', atkr)
     decreases steps1, steps2
 {
     reveal_validEnclaveExecution();
@@ -714,7 +714,7 @@ lemma lemma_validEnclaveEx_enc_conf(s1: state, d1: PageDb, s1':state, d1': PageD
 
     lemma_validEnclaveExecutionStep_validPageDb(s1, d1, s15, d15, dispPg, retToEnclave1);
     lemma_validEnclaveExecutionStep_validPageDb(s2, d2, s25, d25, dispPg, retToEnclave2);
-    lemma_validEnclaveStep_enc_conf(s1, d1, s15, d15, s2, d2, s25, d25,
+    lemma_validEnclaveStep_enc(s1, d1, s15, d15, s2, d2, s25, d25,
         dispPg, atkr, retToEnclave1, retToEnclave2);
 
     assert retToEnclave1 == retToEnclave2;
@@ -722,20 +722,20 @@ lemma lemma_validEnclaveEx_enc_conf(s1: state, d1: PageDb, s1':state, d1': PageD
     if(retToEnclave1) {
         lemma_validEnclaveExecution(s15, d15, s1', d1', dispPg, steps1 - 1);
         lemma_validEnclaveExecution(s25, d25, s2', d2', dispPg, steps2 - 1);
-        lemma_validEnclaveEx_enc_conf(s15, d15, s1', d1', s25, d25, s2', d2',
+        lemma_validEnclaveEx_enc(s15, d15, s1', d1', s25, d25, s2', d2',
                                          dispPg, steps1 - 1, steps2 - 1, atkr);
-        assert enc_conf_eqpdb(d1', d2', atkr);
+        assert enc_eqpdb(d1', d2', atkr);
     } else {
         assert s2' == s25;
         assert s1' == s15;
         assert d1' == d15;
         assert d2' == d25;
-        assert enc_conf_eqpdb(d1', d2', atkr);
+        assert enc_eqpdb(d1', d2', atkr);
     }
 
 }
 
-lemma lemma_validEnclaveStep_enc_conf(s1: state, d1: PageDb, s1':state, d1': PageDb,
+lemma lemma_validEnclaveStep_enc(s1: state, d1: PageDb, s1':state, d1': PageDb,
                                       s2: state, d2: PageDb, s2':state, d2': PageDb,
                                       dispPage:PageNr, atkr: PageNr, ret1:bool, ret2:bool)
     requires ValidState(s1) && ValidState(s2) &&
@@ -745,18 +745,18 @@ lemma lemma_validEnclaveStep_enc_conf(s1: state, d1: PageDb, s1':state, d1': Pag
     requires atkr_entry(d1, d2, dispPage, atkr)
     requires validEnclaveExecutionStep(s1, d1, s1', d1', dispPage, ret1);
     requires validEnclaveExecutionStep(s2, d2, s2', d2', dispPage, ret2);
-    requires enc_conf_eqpdb(d1, d2, atkr)
-    requires enc_conf_eq_entry(s1, s2, d1, d2, atkr)
+    requires enc_eqpdb(d1, d2, atkr)
+    requires s1.conf.nondet == s2.conf.nondet
     requires OperandContents(s1, OLR) == OperandContents(s2, OLR)
     requires user_regs(s1.regs) == user_regs(s2.regs)
     requires mode_of_state(s1) != User && mode_of_state(s2) != User
     requires spsr_same(s1, s2)
     requires s1.conf.scr == s2.conf.scr;
     ensures  atkr_entry(d1', d2', dispPage, atkr)
-    ensures  enc_conf_eqpdb(d1', d2', atkr)
+    ensures  enc_eqpdb(d1', d2', atkr)
     ensures  ret1 == ret2
     ensures  ret1 ==> s1'.conf.scr == s2'.conf.scr;
-    ensures  ret1 ==> enc_conf_eq_entry(s1', s2', d1', d2', atkr)
+    ensures  ret1 ==> s1'.conf.nondet == s2'.conf.nondet
     ensures  ret1 ==> OperandContents(s1', OLR) == OperandContents(s2', OLR)
     ensures  ret1 ==> user_regs(s1'.regs) == user_regs(s2'.regs)
 {
@@ -769,7 +769,7 @@ lemma lemma_validEnclaveStep_enc_conf(s1: state, d1: PageDb, s1':state, d1': Pag
         validEnclaveExecutionStep'(s2, d2, s24, d24, s2', d2',
             dispPage, ret2);
 
-    lemma_validEnclaveStepPrime_enc_conf(
+    lemma_validEnclaveStepPrime_enc(
         s1, d1, s14, d14, s1', d1',
         s2, d2, s24, d24, s2', d2',
         dispPage, ret1, ret2, atkr);
@@ -881,7 +881,7 @@ s21: state, s2':state, s22: state)
     assert evalUpdate(takestep(s2'), OSReg(cpsr), spsr2v, s22);
 }
 
-lemma lemma_validEnclaveStepPrime_enc_conf(
+lemma lemma_validEnclaveStepPrime_enc(
 s11: state, d11: PageDb, s14:state, d14:PageDb, r1:state, rd1:PageDb,
 s21: state, d21: PageDb, s24:state, d24:PageDb, r2:state, rd2:PageDb,
 dispPg:PageNr, retToEnclave1:bool, retToEnclave2:bool, atkr: PageNr
@@ -895,22 +895,22 @@ dispPg:PageNr, retToEnclave1:bool, retToEnclave2:bool, atkr: PageNr
     requires validEnclaveExecutionStep'(s21,d21,s24,d24,r2,rd2,dispPg,retToEnclave2)
     requires OperandContents(s11, OLR) == OperandContents(s21, OLR)
     requires user_regs(s11.regs) == user_regs(s21.regs)
-    requires enc_conf_eqpdb(d11, d21, atkr)
-    requires enc_conf_eq_entry(s11, s21, d11, d21, atkr)
+    requires enc_eqpdb(d11, d21, atkr)
+    requires s11.conf.nondet == s21.conf.nondet
     requires mode_of_state(s11) != User && mode_of_state(s21) != User
     requires spsr_same(s11, s21)
     requires s11.conf.scr == s21.conf.scr;
     ensures  atkr_entry(rd1, rd2, dispPg, atkr)
-    ensures  enc_conf_eqpdb(rd1, rd2, atkr)
+    ensures  enc_eqpdb(rd1, rd2, atkr)
     ensures  retToEnclave1 == retToEnclave2
     ensures  retToEnclave1 ==> r1.conf.scr == r2.conf.scr
-    ensures  retToEnclave1 ==> enc_conf_eq_entry(r1, r2, rd1, rd2, atkr)
+    ensures  retToEnclave1 ==> r1.conf.nondet == r2.conf.nondet
     ensures  retToEnclave1 ==> OperandContents(r1, OLR) == OperandContents(r2, OLR)
     ensures  retToEnclave1 ==> user_regs(r1.regs) == user_regs(r2.regs)
 {                        
 
     assert l1pOfDispatcher(d11, dispPg) == l1pOfDispatcher(d21, dispPg) by
-        { reveal_enc_conf_eqpdb(); }
+        { reveal_enc_eqpdb(); }
     var l1p := l1pOfDispatcher(d11, dispPg);
 
     assert dataPagesCorrespond(s11.m, d11);
@@ -957,7 +957,7 @@ dispPg:PageNr, retToEnclave1:bool, retToEnclave2:bool, atkr: PageNr
 
     var pt1 := ExtractAbsPageTable(s12);
     var pt2 := ExtractAbsPageTable(s22);
-    lemma_userStatesEquiv_atkr_conf(
+    lemma_userStatesEquiv_atkr(
         s11, s1', s12, s14, pc1, pt1, d11,
         s21, s2', s22, s24, pc2, pt2, d21,
         dispPg, atkr, l1p);
@@ -1008,7 +1008,7 @@ dispPg:PageNr, retToEnclave1:bool, retToEnclave2:bool, atkr: PageNr
 
     assert s14.conf.nondet == s24.conf.nondet;
 
-    lemma_userspaceExec_atkr_conf(
+    lemma_userspaceExec_atkr(
         s11, s1', s12, s13, s14, d11, d14,
         s21, s2', s22, s23, s24, d21, d24,
         dispPg, atkr, l1p);
@@ -1055,8 +1055,8 @@ dispPg:PageNr, retToEnclave1:bool, retToEnclave2:bool, atkr: PageNr
         assert r1.conf.nondet == r2.conf.nondet by {
             assert s14.conf.nondet == s24.conf.nondet; 
         }
-        assert enc_conf_eqpdb(rd1, rd2, atkr);
-        assert enc_conf_eq_entry(r1, r2, rd1, rd2, atkr);
+        assert enc_eqpdb(rd1, rd2, atkr);
+        assert r1.conf.nondet == r2.conf.nondet;
         var ret1 := svcHandled(s14, d14, dispPg);
         var ret2 := svcHandled(s24, d24, dispPg);
         assert user_regs(r1.regs) == user_regs(r2.regs) by
@@ -1093,13 +1093,13 @@ dispPg:PageNr, retToEnclave1:bool, retToEnclave2:bool, atkr: PageNr
         assert s24 == exceptionTakenFn(s23, ex2, expc2) by {
             assert evalExceptionTaken(s13, ex1, expc1, s14);
         }
-        lemma_exceptionTaken_atkr_conf(
+        lemma_exceptionTaken_atkr(
             s13, s14, ex1, expc1, 
             s23, s24, ex2, expc2);
-        lemma_exceptionHandled_atkr_conf(s14, d14, rd1, s24, d24, rd2,
+        lemma_exceptionHandled_atkr(s14, d14, rd1, s24, d24, rd2,
              dispPg, atkr);
 
-        assert enc_conf_eqpdb(rd1, rd2, atkr);
+        assert enc_eqpdb(rd1, rd2, atkr);
     }
 }
 
@@ -1117,7 +1117,7 @@ requires ValidState(s1) && ValidState(s2)
     
 }
 
-lemma lemma_exceptionTaken_atkr_conf(
+lemma lemma_exceptionTaken_atkr(
     s13: state, s14: state, ex1:exception, pc1:word,
     s23: state, s24: state, ex2:exception, pc2:word
 )
@@ -1171,13 +1171,13 @@ predicate lr_spsr_same(s1:state, s2:state)
     s1.sregs[spsr(mode_of_state(s1))] == s2.sregs[spsr(mode_of_state(s2))]
 }
 
-lemma lemma_exceptionHandled_atkr_conf(
+lemma lemma_exceptionHandled_atkr(
 s1: state, d1: PageDb, d1': PageDb, s2: state, d2: PageDb, d2': PageDb,
 dispPg: PageNr, atkr: PageNr)
     requires ValidState(s1) && ValidState(s2) &&
              validPageDb(d1') && validPageDb(d2') &&
              validPageDb(d1) && validPageDb(d2) && SaneConstants()
-    requires enc_conf_eq_entry(s1, s2, d1, d2, atkr);
+    requires s1.conf.nondet == s2.conf.nondet;
     requires mode_of_state(s1) != User && mode_of_state(s2) != User
     requires mode_of_state(s1) == mode_of_state(s2)
     requires lr_spsr_same(s1, s2)
@@ -1185,13 +1185,13 @@ dispPg: PageNr, atkr: PageNr)
     requires d1' == exceptionHandled(s1, d1, dispPg).2
     requires d2' == exceptionHandled(s2, d2, dispPg).2
     requires atkr_entry(d1, d2, dispPg, atkr)
-    requires enc_conf_eqpdb(d1, d2, atkr)
+    requires enc_eqpdb(d1, d2, atkr)
     requires user_regs(s1.regs) == user_regs(s2.regs)
     requires s1.conf.ex == s2.conf.ex
-    ensures  enc_conf_eqpdb(d1', d2', atkr)
+    ensures  enc_eqpdb(d1', d2', atkr)
     ensures  atkr_entry(d1', d2', dispPg, atkr)
 {
-    reveal_enc_conf_eqpdb();
+    reveal_enc_eqpdb();
     var ex := s1.conf.ex;
     forall (n : PageNr |  n != dispPg)
         ensures d1'[n] == d1[n];
@@ -1234,7 +1234,7 @@ lemma
     {:fuel userspaceExecutionAndException', 0}
     {:fuel ExtractAbsPageTable, 0}
     {:fuel l1pOfDispatcher, 0}
-lemma_userMemEquiv_atkr_conf(
+lemma_userMemEquiv_atkr(
 s11: state, s1':state, s12: state, s14: state,
 pc1: word, pt1: Maybe<AbsPTable>, d1: PageDb,
 s21: state, s2':state, s22: state, s24: state,
@@ -1245,8 +1245,8 @@ dispPg: PageNr, atkr: PageNr, l1p: PageNr)
     requires validPageDb(d1) && validPageDb(d2)
     requires SaneConstants()
     requires valAddrPage(d1, atkr) && valAddrPage(d2, atkr)
-    requires enc_conf_eqpdb(d1, d2, atkr)
-    requires enc_conf_eq_entry(s12, s22, d1, d2, atkr);
+    requires enc_eqpdb(d1, d2, atkr)
+    requires s12.conf.nondet == s22.conf.nondet
     requires userspaceExecutionAndException'(s11, s1', s12, s14)
     requires userspaceExecutionAndException'(s21, s2', s22, s24)
     requires pc1 == OperandContents(s11, OLR) && pc2 == OperandContents(s21, OLR);
@@ -1290,7 +1290,7 @@ dispPg: PageNr, atkr: PageNr, l1p: PageNr)
     }
 }
 
-lemma lemma_userStatesEquiv_atkr_conf(
+lemma lemma_userStatesEquiv_atkr(
 s11: state, s1':state, s12: state, s14: state,
 pc1: word, pt1: Maybe<AbsPTable>, d1: PageDb,
 s21: state, s2':state, s22: state, s24: state,
@@ -1301,8 +1301,8 @@ dispPg: PageNr, atkr: PageNr, l1p: PageNr)
     requires validPageDb(d1) && validPageDb(d2)
     requires SaneConstants()
     requires valAddrPage(d1, atkr) && valAddrPage(d2, atkr)
-    requires enc_conf_eqpdb(d1, d2, atkr)
-    requires enc_conf_eq_entry(s12, s22, d1, d2, atkr);
+    requires enc_eqpdb(d1, d2, atkr)
+    requires s12.conf.nondet == s22.conf.nondet
     requires userspaceExecutionAndException'(s11, s1', s12, s14)
     requires userspaceExecutionAndException'(s21, s2', s22, s24)
     requires pc1 == OperandContents(s11, OLR) && pc2 == OperandContents(s21, OLR);
@@ -1324,7 +1324,7 @@ dispPg: PageNr, atkr: PageNr, l1p: PageNr)
     ensures pt1.Just? && pt2.Just?
     ensures  user_visible_state(s12, pc1, pt1.v) == user_visible_state(s22, pc2, pt2.v)
 {
-    lemma_userMemEquiv_atkr_conf(
+    lemma_userMemEquiv_atkr(
         s11, s1', s12, s14, pc1, pt1, d1,
         s21, s2', s22, s24, pc2, pt2, d2,
         dispPg, atkr, l1p);
@@ -1370,7 +1370,7 @@ a:addr, atkr:PageNr, l1p: PageNr)
     requires validPageDb(d1) && validPageDb(d2)
     requires ValidState(s1) && ValidState(s2) && SaneConstants()
     requires valAddrPage(d1, atkr) && valAddrPage(d2, atkr)
-    requires enc_conf_eqpdb(d1, d2, atkr)
+    requires enc_eqpdb(d1, d2, atkr)
     requires dataPagesCorrespond(s1.m, d1) && dataPagesCorrespond(s2.m, d2)
     requires ExtractAbsPageTable(s1).Just?
     requires ExtractAbsPageTable(s2).Just?
@@ -1414,12 +1414,12 @@ n:PageNr, a:addr, atkr:PageNr)
     requires d2[n].PageDbEntryTyped? && d2[n].entry.DataPage?
     requires valAddrPage(d1, atkr) && valAddrPage(d2, atkr)
     requires d1[n].addrspace == atkr && d2[n].addrspace == atkr
-    requires enc_conf_eqpdb(d1, d2, atkr)
+    requires enc_eqpdb(d1, d2, atkr)
     requires a in addrsInPage(n, page_monvaddr(n))
     requires dataPagesCorrespond(s1.m, d1) && dataPagesCorrespond(s2.m, d2)
     ensures s1.m.addresses[a] == s2.m.addresses[a]
 {
-    reveal enc_conf_eqpdb();
+    reveal enc_eqpdb();
     reveal pageDbDataCorresponds();
 
     // trigger i in pageDbDataCorresponds:
@@ -1434,7 +1434,7 @@ l1p:PageNr, atkr: PageNr)
     requires ValidState(s1) && ValidState(s2) && SaneConstants()
     requires valAddrPage(d1, atkr) && valAddrPage(d2, atkr)
     requires !stoppedAddrspace(d1[atkr]) && !stoppedAddrspace(d2[atkr])
-    requires enc_conf_eqpdb(d1, d2, atkr)
+    requires enc_eqpdb(d1, d2, atkr)
     requires nonStoppedL1(d1, l1p) && nonStoppedL1(d2, l1p)
     requires pageTableCorresponds(s1, d1, l1p)
     requires pageTableCorresponds(s2, d2, l1p)
@@ -1445,7 +1445,7 @@ l1p:PageNr, atkr: PageNr)
 {
     reveal pageTableCorresponds();
     assert mkAbsPTable(d1, l1p) == mkAbsPTable(d2, l1p) by {
-        reveal enc_conf_eqpdb();
+        reveal enc_eqpdb();
         reveal validPageDb();
         reveal mkAbsPTable();
     }
@@ -1454,19 +1454,19 @@ l1p:PageNr, atkr: PageNr)
 //-----------------------------------------------------------------------------
 // Resume
 //-----------------------------------------------------------------------------
-lemma lemma_resume_enc_conf_ni(s1: state, d1: PageDb, s1':state, d1': PageDb,
+lemma lemma_resume_enc_ni(s1: state, d1: PageDb, s1':state, d1': PageDb,
                                s2: state, d2: PageDb, s2':state, d2': PageDb,
                                dispPage: word,
                                atkr: PageNr)
     requires ni_reqs(s1, d1, s1', d1', s2, d2, s2', d2', atkr)
     requires smc_resume(s1, d1, s1', d1', dispPage)
     requires smc_resume(s2, d2, s2', d2', dispPage)
-    requires enc_conf_eqpdb(d1, d2, atkr)
+    requires enc_eqpdb(d1, d2, atkr)
     requires entering_atkr(d1, d2, dispPage, atkr, true) ==>
-        enc_conf_eq_entry(s1, s2, d1, d2, atkr)
-    ensures enc_conf_eqpdb(d1', d2', atkr)
+        s1.conf.nondet == s2.conf.nondet
+    ensures enc_eqpdb(d1', d2', atkr)
 {
-    reveal_enc_conf_eqpdb();
+    reveal_enc_eqpdb();
     if(!validPageNr(dispPage)){
         assert d1' == d1 &&  d2' == d2;
     } else {
@@ -1477,8 +1477,8 @@ lemma lemma_resume_enc_conf_ni(s1: state, d1: PageDb, s1':state, d1': PageDb,
             assert d2[dispPage].PageDbEntryTyped?;
             var asp1, asp2 := d1[dispPage].addrspace, d2[dispPage].addrspace;
             var e1', e2' := smc_enter_err(d1, dispPage, true), smc_enter_err(d2, dispPage, true);
-            assert enc_conf_eqpdb(d1', d2', atkr) by {
-                lemma_enter_enc_conf_eqpdb(s1, d1, s1', d1', s2, d2, s2', d2',
+            assert enc_eqpdb(d1', d2', atkr) by {
+                lemma_enter_enc_eqpdb(s1, d1, s1', d1', s2, d2, s2', d2',
                                  dispPage, 0, 0, 0, asp1, asp2, atkr, 
                                  true);
             }
@@ -1494,7 +1494,7 @@ lemma lemma_resume_enc_conf_ni(s1: state, d1: PageDb, s1':state, d1': PageDb,
                 assert e1' == KOM_ERR_SUCCESS <==> e2' == KOM_ERR_SUCCESS;
                 if(e1' == KOM_ERR_SUCCESS) {
                     assert entering_atkr(d1, d2, dispPage, atkr, true);
-                    lemma_enter_enc_conf_atkr_enter(s1, d1, s1', d1', s2, d2, s2', d2',
+                    lemma_enter_enc_atkr_enter(s1, d1, s1', d1', s2, d2, s2', d2',
                                                     dispPage, 0, 0, 0, 
                                                     atkr, true);
                 } else {
